Add min_full_ts

src/lang/Cell.v
@@ -1365,4 +1365,120 @@ Module Cell.
     - exploit COMPLETE; eauto. i. des.
       esplits; eauto.
   Qed.
+
+
+  (* min_full_ts *)
+
+  Inductive min_full_ts (cell: t) (ts: Time.t): Prop :=
+  | min_full_ts_intro
+      (GET: exists from val released, get ts cell = Some (from, Message.full val released))
+      (MIN: forall to from' val' released'
+              (GET: get to cell = Some (from', Message.full val' released')),
+          Time.le ts to)
+  .
+
+  Lemma min_full_ts_exists_aux
+        A t a
+        (l: list (Time.t * A))
+        (f: A -> bool)
+        (INHABITED1: f a = true)
+        (INHABITED2: List.In (t, a) l):
+    exists min_t min_a,
+      f min_a = true /\
+      List.In (min_t, min_a) l /\
+      (forall t' a' (IN: List.In (t', a') l) (F: f a' = true), Time.le min_t t').
+  Proof.
+    remember (length l) eqn:LEN.
+    revert INHABITED1 INHABITED2 LEN. revert t a l.
+    induction n; i.
+    { destruct l; inv LEN. inv INHABITED2. }
+    destruct l; inv LEN.
+    destruct p as [t1 a1]. ss. des.
+    - inv INHABITED2. destruct l.
+      + esplits; eauto. i. des; inv IN. refl.
+      + exploit (IHn t0 a ((t0, a)::l)); auto; try by econs.
+        i. des. destruct p as [new_t new_a]. ss.
+        destruct (f new_a) eqn:FNEW; cycle 1.
+        { esplits; try exact x0.
+          - des; eauto.
+          - i. guardH x1. des.
+            + inv IN. eapply x2; eauto.
+            + inv IN. rewrite F in FNEW. inv FNEW.
+            + eapply x2; eauto. }
+        destruct (Time.le_lt_dec min_t new_t).
+        { esplits; try exact x0.
+          - des; eauto.
+          - i. guardH x1. des.
+            + inv IN. eapply x2; eauto.
+            + inv IN. auto.
+            + eapply x2; eauto. }
+        exists new_t. exists new_a. splits; auto.
+        i. guardH x1. des.
+        * inv IN. exploit (x2 t' a'); eauto. i.
+          etrans; eauto. econs. auto.
+        * inv IN. refl.
+        * etrans; [econs; try exact l0|].
+          eapply x2; eauto.
+    - exploit (IHn t0 a l); eauto. i. des.
+      destruct (f a1) eqn:FNEW; cycle 1.
+      { esplits; try exact x0; eauto.
+        i. des.
+        - inv IN. rewrite FNEW in F. inv F.
+        - eapply x2; eauto. }
+      destruct (Time.le_lt_dec min_t t1).
+      { esplits; try exact x0; eauto.
+        i. des.
+        - inv IN. auto.
+        - eapply x2; eauto. }
+      exists t1. exists a1. esplits; eauto.
+      i. des.
+      + inv IN. refl.
+      + etrans; [econs; exact l0|].
+        eapply x2; eauto.
+  Qed.
+
+  Lemma min_full_ts_exists
+        from to val released cell
+        (INHABITED: get to cell = Some (from, Message.full val released)):
+    exists ts, min_full_ts cell ts.
+  Proof.
+    destruct cell. unfold get in *. ss.
+    remember (DOMap.elements raw0) as l eqn:DOM.
+    exploit (min_full_ts_exists_aux
+               to (from, Message.full val released) l
+               (fun (a: Time.t * Message.t) => match a with
+                                            | (_, Message.full _ _) => true
+                                            | _ => false
+                                            end)).
+    { ss. }
+    { subst. eapply DOMap.elements_correct. auto. }
+    i. des. destruct min_a. destruct t1; ss.
+    exists min_t. econs.
+    - subst. esplits. unfold get. ss.
+      eapply DOMap.elements_complete. eauto.
+    - i. unfold get in GET. ss.
+      apply DOMap.elements_correct in GET. subst.
+      eapply x2; eauto.
+  Qed.
+
+  Lemma min_full_ts_inj
+        cell ts1 ts2
+        (MIN1: min_full_ts cell ts1)
+        (MIN2: min_full_ts cell ts2):
+    ts1 = ts2.
+  Proof.
+    inv MIN1. inv MIN2. des.
+    apply MIN0 in GET. apply MIN in GET0.
+    apply TimeFacts.antisym; auto.
+  Qed.
+
+  Lemma min_full_ts_spec
+        ts from val released cell mts
+        (MIN: min_full_ts cell mts)
+        (GET: get ts cell = Some (from, Message.full val released)):
+    <<GET: exists f v r, get mts cell = Some (f, Message.full v r)>> /\
+    <<MIN: Time.le mts ts>>.
+  Proof.
+    inv MIN. des. esplits; eauto.
+  Qed.
 End Cell.
