src/lang/Memory.v
@@ -2972,4 +2972,37 @@ Module Memory.
     - exploit remove_get1; try exact GET; eauto. i. des; eauto.
       subst. exploit remove_get0; try exact MEM. i. des. congr.
   Qed.
+
+
+  (* lemmas on min_full_ts *)
+
+  Definition min_full_ts (mem: t) (loc: Loc.t) (ts: Time.t): Prop :=
+    Cell.min_full_ts (mem loc) ts.
+
+  Lemma min_full_ts_exists
+        mem loc
+        (INHABITED: inhabited mem):
+    exists ts, min_full_ts mem loc ts.
+  Proof.
+    eapply Cell.min_full_ts_exists. apply INHABITED.
+  Qed.
+
+  Lemma min_full_ts_inj
+        mem loc ts1 ts2
+        (MIN1: min_full_ts mem loc ts1)
+        (MIN2: min_full_ts mem loc ts2):
+    ts1 = ts2.
+  Proof.
+    eapply Cell.min_full_ts_inj; eauto.
+  Qed.
+
+  Lemma min_full_ts_spec
+        loc ts from val released mem mts
+        (MIN: min_full_ts mem loc mts)
+        (GET: get loc ts mem = Some (from, Message.full val released)):
+    <<GET: exists from val' released', get loc mts mem = Some (from, Message.full val' released')>> /\
+    <<MIN: Time.le mts ts>>.
+  Proof.
+    eapply Cell.min_full_ts_spec; eauto.
+  Qed.
 End Memory.
